WIP

SSA/Projects/InstCombine/Bug.lean
@@ -3,6 +3,7 @@ import SSA.Projects.InstCombine.LLVM.EDSL
 import SSA.Projects.InstCombine.AliveStatements
 import SSA.Projects.InstCombine.Refinement
 import SSA.Projects.InstCombine.Tactic
+import SSA.Core.Tactic
 import SSA.Projects.InstCombine.ComWrappers
 
 open MLIR AST
@@ -10,8 +11,28 @@ open Std (BitVec)
 open Ctxt (Var)
 open ComWrappers
 
-set_option pp.proofs true
-set_option pp.proofs.withType true
+macro "simp_alive_meta" : tactic =>
+  `(tactic|
+      (
+        simp only [InstcombineTransformDialect.MOp.instantiateCom,
+                   InstcombineTransformDialect.instantiateMTy,
+                   InstcombineTransformDialect.instantiateMOp,
+                   Expr.mk,
+                   ConcreteOrMVar.instantiate,
+                   Vector.get,
+                   List.nthLe,
+                   List.get,
+                   InstCombine.MTy.bitvec,
+                   DialectMorphism.mapTy
+        ] at *
+      )
+  )
+
+
+--set_option pp.proofs true
+--set_option pp.proofs.withType true
+--set_option pp.all true
+--set_option pp.explicit true
 set_option linter.deprecated false
 
 def src_i1 (w : Nat) :=
@@ -33,38 +54,36 @@ def tgt  (w : Nat)  :=
   "llvm.return" (%v1) : (_) -> ()
 }]
 
-def src_cw (w : Nat) :
+def src_i1_cw :
   Com InstCombine.Op [InstCombine.Ty.bitvec 1] (InstCombine.Ty.bitvec 1) :=
   .ret ⟨0, by simp [Ctxt.snoc]⟩
 
-def src_i1_cw (w : Nat) :
+def src_cw (w : Nat) :
   Com InstCombine.Op [InstCombine.Ty.bitvec w] (InstCombine.Ty.bitvec w) :=
   .ret ⟨0, by simp [Ctxt.snoc]⟩
 
 def tgt_cw (w : Nat) :
   Com InstCombine.Op [InstCombine.Ty.bitvec w] (InstCombine.Ty.bitvec w) :=
   .lete (ComWrappers.mul w 0 0) <|
-  .ret ⟨1, by simp [Ctxt.snoc]⟩
+  .ret ⟨0, by simp [Ctxt.snoc]⟩
 
 def src_cw_hidden (w : Nat) := src_cw w
 def src_i1_cw_hidden (w : Nat) := src_cw w
 
-#check src_cw 1
-#check src_i1_cw 1
-#check src 1
-#check src_i1 1
-#check tgt 1
-
 theorem ss : src_i1 1 = src 1 := rfl
 theorem sss : src_cw 1 = src 1 := rfl
-theorem ssss : src_i1_cw 1 = src 1 := rfl
+theorem ssss : src_i1_cw = src 1 := rfl
+
+theorem tgttt : tgt_cw 1 = tgt 1 := rfl
 
 open Ctxt
 
 /-- This one does not have the 'snoc' leftover. -/
-theorem okkk : src_cw_hidden 1  ⊑ tgt 1  := by
-  unfold tgt
-
+theorem okkk : src_cw 1  ⊑ tgt_cw 1  := by
+  unfold tgt_cw
+  unfold src_cw
+  unfold mul
+  simp_alive_ssa
   dsimp only [Com.Refinement]
   intros Γv
   change_mlir_context Γv
@@ -75,13 +94,17 @@ theorem okkk : src_cw_hidden 1  ⊑ tgt 1  := by
   simp (config := {failIfUnchanged := false}) only [HVector.map]
   simp (config := {failIfUnchanged := false}) only [List.map_eq_map]
   simp (config := {failIfUnchanged := false}) only [Var.zero_eq_last]
-  rw [Valuation.snoc_last]
+  simp only [Valuation.snoc_last]
   sorry
 
 
 /-- This one does not have the 'snoc' leftover. -/
-theorem okk : src_i1_cw_hidden 1  ⊑ tgt 1  := by
-  unfold tgt
+theorem okk : src_i1_cw  ⊑ tgt_cw 1  := by
+  unfold tgt_cw
+  unfold src_i1_cw
+  unfold mul
+
+  simp_alive_ssa
   dsimp only [Com.Refinement]
   intros Γv
   change_mlir_context Γv
@@ -92,8 +115,10 @@ theorem okk : src_i1_cw_hidden 1  ⊑ tgt 1  := by
   simp (config := {failIfUnchanged := false}) only [HVector.map]
   simp (config := {failIfUnchanged := false}) only [List.map_eq_map]
   simp (config := {failIfUnchanged := false}) only [Var.zero_eq_last]
-  rw [Valuation.snoc_last]
+  simp only [Valuation.snoc_last]
   sorry
+
+#check Lean.Meta.Simp.Config
 
 /-- This one does not have the 'snoc' leftover. -/
 theorem ok : src 1  ⊑ tgt 1  := by
@@ -101,20 +126,18 @@ theorem ok : src 1  ⊑ tgt 1  := by
   dsimp only [Com.Refinement]
   intros Γv
   change_mlir_context Γv
-
   simp (config := {failIfUnchanged := false}) only [Com.denote]
   simp (config := {failIfUnchanged := false}) only [Expr.denote]
   simp (config := {failIfUnchanged := false}) only [HVector.denote]
   simp (config := {failIfUnchanged := false}) only [HVector.map]
   simp (config := {failIfUnchanged := false}) only [List.map_eq_map]
   simp (config := {failIfUnchanged := false}) only [Var.zero_eq_last]
-  rw [Valuation.snoc_last]
+  simp only [Valuation.snoc_last]
   sorry
 
 /-- This one has the 'snoc' leftover. -/
 theorem broken : src_i1 1 ⊑ tgt 1  := by
   unfold tgt
-  -- Γv✝ : Ctxt.Valuation [InstCombine.MTy.bitvec (ConcreteOrMVar.concrete 1)]
   -- ∀ (e : Option (_root_.BitVec 1)),
   -- Com.denote (src_i1 1) Γv✝ ⊑ Ctxt.Valuation.snoc Γv✝ (LLVM.mul e e) { val := 0, property := ⋯ }
   dsimp only [Com.Refinement]
@@ -127,5 +150,31 @@ theorem broken : src_i1 1 ⊑ tgt 1  := by
   simp (config := {failIfUnchanged := false}) only [HVector.map]
   simp (config := {failIfUnchanged := false}) only [List.map_eq_map]
   simp (config := {failIfUnchanged := false}) only [Var.zero_eq_last]
-  rw [Valuation.snoc_last] -- <= This one does not fire!
+  simp_alive_meta
+  simp [InstcombineTransformDialect.instantiateMTy]
+  --set_option trace.Meta.isDefEq true in
+  rw [Valuation.snoc_last]
   sorry
+
+
+def alive_Select_858_src  (w : Nat)   :=
+[alive_icom ( w )| {
+^bb0(%a : i1, %b : i1):
+  %v1 = "llvm.mlir.constant" () { value = -1 : i1 } :() -> (i1)
+  %v2 = "llvm.xor" (%a,%v1) : (i1, i1) -> (i1)
+  %v3 = "llvm.select" (%a,%v2,%b) : (i1, i1, i1) -> (i1)
+  "llvm.return" (%v3) : (i1) -> ()
+}]
+
+def alive_Select_858_tgt  (w : Nat)  :=
+[alive_icom ( w )| {
+^bb0(%a : _, %b : _):
+  %v1 = "llvm.mlir.constant" () { value = -1 : _ } :() -> (_)
+  %v2 = "llvm.xor" (%a,%v1) : (_, _) -> (_)
+  %v3 = "llvm.and" (%v2,%b) : (_, _) -> (_)
+  "llvm.return" (%v3) : (_) -> ()
+}]
+theorem alive_Select_858  (w : Nat)   : alive_Select_858_src w  ⊑ alive_Select_858_tgt 1  := by
+  unfold alive_Select_858_src alive_Select_858_tgt
+  simp_alive_peephole -- fails to clear the context
+  all_goals sorry --apply bitvec_Select_858
